# Theorem 1.19

$$(-1)^{2k} = ((-1)^2)^k = 1^k = 1$$

$(2k)!$ has $2k$ terms, and can therefore be also written as
$$(2k)! = (-1)(-2)\cdots(-2k + 1)(-2k)$$

Now finally note that $-a \equiv p - a \mod p$, and the expression
becomes $(p - 1)! \mod p$.

## Wilson's Theorem

Wilson's theorem in short:

$\mathbb{Z}_p$ is a field so all $x \in \mathbb{Z}_p^* = \mathbb{Z}_p \setminus \{ 0 \}$ is a unit
$\implies \bar{2} \cdot \overline{p - 2} = \bar{1}$
\begin{align*}
(p - 1)! &\equiv (p - 1)(p - 2)! \mod p \\
    &\equiv -1 \cdot 1 \mod p
\end{align*}

See also Pinter, 23G.

# Lemma 1.28

The only units in $\mathbb{Z}[i]$ are $\pm 1, \pm i$.

