# Exercise 3.15

Verify that if $K = \mathbb{Q}(\sqrt{-2}, \sqrt{-5})$ then an integral basis is given
by $\{ 1, \sqrt{-2}, \sqrt{-5}, \frac{\sqrt{-2} + \sqrt{10}}{2} \}$.

See proposition 2.34 that integral elements of $\mathbb{Z}[\sqrt{d}]$ have the form
$\mathbb{Z} + \mathbb{Z}\sqrt{d}$ when $d \equiv 2, 3 \mod 4$.

Adding $\alpha$ with its conjugates creates elements of the form $2a + 2k\sqrt{d} \in \mathbb{Z}_K$
where $d \in \{ -2, -5, 10 \}$. $-2 \equiv 2 \mod 4, -5 \equiv 3 \mod 4, 10 \equiv 2 \mod 4$.
So we know by above that these elements are from $\mathbb{Z} + \mathbb{Z}\sqrt{d}$.
So $2a, 2k \in \mathbb{Z}$.

Follow method of previous section.

$$A = 2a, B = 2b, C = 2c, D = 2d \in \mathbb{Z}$$
$$a = \frac{A}{2}, b = \frac{B}{2}, c = \frac{C}{2}, d = \frac{D}{2}$$

\begin{align*}
\alpha &= a + b\sqrt{-2} + c\sqrt{-5} + d\sqrt{10} \\
    &= \frac{A}{2} + \frac{B}{2}\sqrt{-2} + \frac{C}{2}\sqrt{-5} + \frac{D}{2}\sqrt{10} \\
\alpha_2 &= a - b \sqrt{-2} + c\sqrt{-5} - d\sqrt{10} \\
\alpha \alpha_2 &= ((a + c\sqrt{-5}) - (b\sqrt{-2} + d\sqrt{10}))((a + c\sqrt{-5}) + (b\sqrt{-2} + d\sqrt{10})) \\
    &= (a + c\sqrt{-5})^2 - (b\sqrt{-2} + d\sqrt{10})^2 \\
    &= a^2 + 2\sqrt{-5}ac - 5c^2 + 2b^2 - 2\sqrt{-20}bd - 10d^2 \\
    &= \frac{A^2 - 5C^2 + 2B^2 - 10D^2}{4} + \frac{AC - 2BD}{2}\sqrt{-5}
\end{align*}

First note that $AC - 2BD \equiv AC \equiv 0 \mod 2$, which means either A or C are even.

\begin{align*}
A^2 - 5C^2 + 2B^2 - 10D^2 &\equiv 0 \mod 2 \\
    &\equiv A^2 - 5C^2 \mod 2 \\
    &\equiv A + C \mod 2
\end{align*}

| $A \mod 2$ | $C \mod 2$ | $A + C \mod 2$ |
|------------|------------|----------------|
| 0          | 0          | 0              |
| 0          | 1          | 1              |
| 1          | 0          | 1              |

So $A$ and $C$ are both even.

Now we look at $B$ and $D$. Note that by the last step
$A^2 \equiv 0 \mod 4$ and $C^2 \equiv 0 \mod 4$.

$$A^2 - 5C^2 + 2B^2 - 10D^2 \equiv 2B^2 - 10D^2 \equiv 0 \mod 4$$
$$2B^2 - 10D^2 = 4p \implies B^2 - 5D^2 = 2p$$
$$B^2 - 5D^2 \equiv B^2 + D^2 \equiv 0 \mod 2$$
$$\implies B + D \equiv 0 \mod 2$$

| $B \mod 2$ | $D \mod 2$ | $B + D \mod 2$ |
|------------|------------|----------------|
| 0          | 0          | 0              |
| 0          | 1          | 1              |
| 1          | 0          | 1              |
| 1          | 1          | 0              |

So $B \equiv D \equiv 0 \mod 2$ or $B \equiv D \equiv 1 \mod 2$.
Remembering $A \equiv C \equiv 0 \mod 2$, we now have 2 cases.

## Case 1: A, B, C, D are all even

$$A \equiv C \equiv 0 \mod 2$$
$$B \equiv D \equiv 0 \mod 2$$

$$A = 2a, B = 2b, C = 2c, D = 2d \in \mathbb{Z}$$

Earlier we found
$$2\alpha = A + B\sqrt{-2} + C\sqrt{-5} + D\sqrt{10}$$
with $A, B, C, D \in \mathbb{Z}$.

But now we know $A, B, C, D \in 2 \mathbb{Z}$.
So $a, b, c, d \in \mathbb{Z}$.

Which is integral over $\{1, \sqrt{-2}, \sqrt{-5}, \sqrt{10}\}$
and so also over $\{1, \sqrt{-2}, \sqrt{-5}, \frac{\sqrt{-2} + \sqrt{10}}{2}\}$
since $\sqrt{10} = 0 \cdot 1 - 1 \cdot \sqrt{-2} + 0 \sqrt{-5} + 2 \frac{\sqrt{-2} + \sqrt{10}}{2}$

## Case 2: A, B are even, C, D are odd

Now we do the other case.

$$A \equiv C \equiv 0 \mod 2$$
$$B \equiv D \equiv 1 \mod 2$$

$$A = 2a, B = 2b, C = 2c, D = 2d$$

Here $A, C \in 2 \mathbb{Z}$ so $a, c \in \mathbb{Z}$.
But this is not true for $B, D$ which are odd integers.

$a, c$ are integers, but $b, d$ are halves of odd integers.
$$\alpha = a + b\sqrt{-2} + c\sqrt{-5} + d\sqrt{10}$$
which has as basis
$\{1, \sqrt{-2}, \sqrt{-5}, \frac{\sqrt{-2} + \sqrt{10}}{2}\}$

So we managed to reduce all elements of $\mathbb{Z}_K$ which both have the same basis.
We therefore conclude that the entire ring has that integral basis too.

# Prove that $\mathbb{Z}_K \neq \mathbb{Z}[\gamma]$

$$\gamma = \frac{\sqrt{-2} + \sqrt{10}}{2}$$

```python
sage: var("a b c d")
(a, b, c, d)
sage: y = (sqrt(-2) + sqrt(10))/2
sage: e = a + b*y + c*y^2 + d*y^3 == 0
sage: e = e.expand()
sage: e
1/2*sqrt(10)*sqrt(-2)*c + 1/2*sqrt(10)*b + 1/2*sqrt(-2)*b + 1/2*sqrt(10)*d + 7/2*sqrt(-2)*d + a + 2*c == 0
```

$$\frac{1}{2} \, \sqrt{10} \sqrt{-2} c + \frac{1}{2} \, \sqrt{10} b + \frac{1}{2} \, \sqrt{-2} b + \frac{1}{2} \, \sqrt{10} d + \frac{7}{2} \, \sqrt{-2} d + a + 2 \, c = 0$$
Tidying up
$$\frac{1}{2} \sqrt{-2} \sqrt{-5} \sqrt{-2} c + \frac{1}{2} \sqrt{10} b + \frac{1}{2} \sqrt{-2} b + \frac{1}{2} \sqrt{10} d + \frac{7}{2} \sqrt{-2} d + a + 2 \, c = 0$$
$$a + 2c + \frac{1}{2} \sqrt{-2} b  + \frac{7}{2} \sqrt{-2} d - \sqrt{-5} c + \frac{1}{2} \sqrt{10} b + \frac{1}{2} \sqrt{10} d = 0$$
$$(a + 2c) + \left(\frac{b + 7d}{2}\right) \sqrt{-2} - c \sqrt{-5} + \frac{b + d}{2} \sqrt{10} = 0$$

We will now search for basis elements which cannot be computed from powers of $\gamma$.
We can use the last equation before to convert elements from the basis $\{ 1, \gamma, \gamma^2, \gamma^3 \}$ to
$\{1, \sqrt{-2}, \sqrt{-5}, \sqrt{10} \}$. We are interested to in reverse, and see if there are elements from
the $\langle \sqrt{-2}, \sqrt{-5} \rangle$ basis to $\langle \gamma \rangle$.

Let $M$ be a 4x4 matrix transform that takes the basis for $\langle \gamma \rangle$ to $\langle \sqrt{-2}, \sqrt{-5} \rangle$.
$$M\bf{v} = A$$
$A$ is the result of the change of basis. So we can actually compute values from $\langle sqrt{-2}, sqrt{-5} \rangle$ in terms
of $\gamma$. But these elements must be integers, otherwise it is not $\mathbb{Z}[\gamma]$.

$$ \begin{pmatrix}
    1 & 0 & 2 & 0 \\
    0 & 1 & 0 & 7 \\
    0 & 0 & 1 & 0 \\
    0 & 1 & 0 & 1 \\
\end{pmatrix}
\begin{pmatrix}
    a \\
    b \\
    c \\
    d \\
\end{pmatrix}
=
\begin{pmatrix}
    a + 2c \\
    b + 7d \\
    c \\
    b + d \\
\end{pmatrix}
$$

where $A$ is our basis. We are interested in

$$ \begin{pmatrix}
    0 \\
    2 \\
    0 \\
    0 \\
\end{pmatrix}
,
\begin{pmatrix}
    0 \\
    0 \\
    -1 \\
    0 \\
\end{pmatrix}
,
\begin{pmatrix}
    0 \\
    0 \\
    0 \\
    2 \\
\end{pmatrix}
$$
Which correspond to the basis over $\langle \sqrt{-2}, \sqrt{-5} \rangle$.
$$(a + 2c) + \left(\frac{b + 7d}{2}\right) \sqrt{-2} - c \sqrt{-5} + \frac{b + d}{2} \sqrt{10} = 0$$

Trying the first one, we get

```python
sage: M = matrix([
....:     [1, 0, 2, 0],
....:     [0, 1, 0, 7],
....:     [0, 0, 1, 0],
....:     [0, 1, 0, 1]
....: ])
sage: v = vector([0, 2, 0, 0])
sage: M^-1*v
(0, -1/3, 0, 1/3)
```
So therefore $\sqrt{-2} \notin \mathbb{Z}[\gamma]$.

# Exercise 3.16

$$f(\gamma) = 0$$
$$3 \mid g(\gamma) \implies g(\gamma) \equiv 0 \mod 3$$
$$g(X) \equiv f(X) u(X) \mod 3$$
likewise
$$g(X) \equiv f(X) u(X) \mod 3$$
$$\implies g(\gamma) \equiv f(\gamma) u(\gamma) \equiv 0 \mod 3$$

$$g(X) = 3a(X) + f(X)u(X)$$

