# Units

## $d â‰¡ 2, 3 \mod 4$

$$N(Î±) = aÂ² - dbÂ² = 1$$

Note $d < 0$ so either $aÂ² = 1$ or $-dbÂ² = 1$.

$$a = Â±1$$

When $d = -1$, then $b = Â±1$ so we also have $Â±i$.

## $d â‰¡ 1 \mod 4$

$$N(Î±) = 1 â‡” (2a + b)Â² - dbÂ² = 4$$
$$d = -3, -7, -11, â€¦$$
We cannot have $-dbÂ² â‰¤ 4$ for $d < -3$, so $b = 0$.
$$(2a + 0) = 4 â‡’ a = Â±1$$

Now consider $d = -3$. $|b| â‰¥ 2 â‡’ -dbÂ² â‰¥ 12$.
So $b = -1, 0, 1$.
Then by solving we find all units for $d = -3$ are
the 6th roots of unity.

## Summary

Note $\bar{Ï‰} = Ï‰^{n - 1}$ so $N(Ï‰) = Ï‰ \bar{Ï‰} = Ï‰^n$.

# Euclidean Imaginary Quadratic Fields

See `ch6-euclid.py`. With $d = -19$, the top vertex becomes
$1.14i$.
$$ N\left(\frac{Î±}{Î²} - Îº\right) > 1 â‡’ N(Ï) = N(Î± - ÎºÎ²) > N(Î²) $$
Let $Î± = 28 \sqrt{d}, Î² = 108$, then $Î±/Î² = 1.13i$. Then we
can confirm the above is true.

## $x = qu + r$ for $u$ a non unit, and $r = 0$ or $r$ a unit

$I$ is the maximal ideal containing all non units of $R$.
Let $u âˆˆ I$ such that $ğœ™(u)$ is minimal in $I$. Then
$$ x = qu + r \textrm{ with } ğœ™(r) < ğœ™(u) \textrm{ or } r = 0 $$
If $r = 0$, then $x = qu$. So assume $r â‰  0$.

$r âˆ‰ I$ because $ğœ™(u)$ is minimal, so $r$ is a unit.

## $â„¤_K$ is not Euclidean

By previous result, $u | Î±$ or $u | 2 Â± 1$.

$u$ cannot divide $1$ since it is not a unit, so $u | 2$ or $3$.

$$ N\left(a + b\left(\frac{1 + \sqrt{d}}{2}\right)\right) = aÂ² + ab + bÂ² \left(\frac{1 - d}{4}\right) $$

$d < -11 â‡’ k = \frac{1 - d}{4} â‰¥ 4$.

$$ aÂ² + ab + kbÂ² = 2, 3 $$
Complete the square and see there's no solution. So both $2, 3$ are irreducible.
$u = 2, -2, 3, -3$.

Now let $Î± = \frac{1 + \sqrt{d}}{2}$, but $u \nmid Î±$ and $u \nmid Î± Â± 1$.
So $u$ does not exist.

# Quadratic Forms

Positive definite forms $f(x, y) â‰¥ 0$ and
$f(x, y) = 0 â‡’ (x, y) = (0, 0)$.

Therefore $a, c > 0$ since $f(x, 0), f(0, y) > 0$.
Complete the square to see $bÂ² - 4ac < 0$.
$$ axÂ² + bxy + cyÂ² = a\left(x + \frac{b}{2a} y\right)Â² + \left(c - \frac{bÂ²}{4a}\right) yÂ² $$

A form is normal if $-a < b â‰¤ a$.

A form is reduced if it is normal and $a < c$ or $a = c$ and $b â‰¥ 0$.

Generators for $\textrm{SL}â‚‚(â„¤)$
$$
T =
\begin{pmatrix}
1 & 1 \\
0 & 1
\end{pmatrix}
\qquad \textrm{and} \qquad
S = \begin{pmatrix}
0 & 1 \\
-1 & 0
\end{pmatrix}
$$
Which correspond to
$$ (a, b + 2a, c + b + a) \qquad \textrm{and} \qquad (c, -b, a) $$

# Minimum Values

$(x, y)$ are coprime.

$$ |x| â‰¥ 2 â‡’ f(x, y) > c $$
$$ |y| â‰¥ 2 â‡’ f(x, y) > c $$

| $x$ | $y$ | $f(x, y)$ |
|-----|-----|-----------|
| -1  | -1  | $> c$     |
| -1  | 0   | $a$       |
| -1  | 1   | $â‰¥ c$     |
| 0   | -1  | $c$       |
| 0   | 1   | $c$       |
| 1   | -1  | $â‰¥ c$     |
| 1   | 0   | $a$       |
| 1   | 1   | $> c$     |

When $a = c$, there are 4 pairs $f(x, y) = a$,
which becomes 6 when $a = b = c$.

## $|y| = 1, |x| â‰¥ 2$

Complete the square
\begin{align*}
4a f(x, y) &= 4a(axÂ² + bxy + cyÂ²) \\
           &= (2ax + by)Â² - (bÂ² - 4ac) yÂ² \\
           &= (2ax + by)Â² - (bÂ² - 4ac)
\end{align*}
But note that
$$ |2ax + by| â‰¥ |2ax| - |by| â‰¥ 4a - |b| â‰¥ 3a $$
since $|y| = 1$ and $b â‰¤ a$.
$$ â‡’ 4a f(x, y) â‰¥ 9aÂ² - (bÂ² - 4ac) = 4ac + 8aÂ² + (aÂ² - bÂ²) $$
but $|b| â‰¤ a$ so $4a f(x, y) â‰¥ 4ac$ or
$$ f(x, y) â‰¥ c $$

## $|y| â‰¥ 2$

$$ 4a f(x, y) = (2ax + by)Â² - (bÂ² - 4ac) yÂ² â‰¥ -(bÂ² - 4ac) yÂ² $$
$$ yÂ² â‰¥ 4 $$
$$ â‡’ 4a f(x, y) â‰¥ -4(bÂ² - 4ac) = 16ac - 4bÂ² $$
Note $bÂ² - 4ac < 0$ and we can factor that out.
$$ 4a f(x, y) â‰¥ 12ac + 4(ac - bÂ²) â‰¥ 12ac â‰¥ 4ac $$
$$ f(x, y) > c $$

## Remaining Cases

$(x, y) = 1$ and if $y = 0$, then $x = Â±1$ so
$$ f(Â±1, 0) = a $$

$$ f(0, Â±1) = c $$
$$ f(Â±1, Â±1) = a + b + c > c $$
$$ f(Â±1, âˆ“1) = a - b + c â‰¥ c $$

# Decompose $M \in \textrm{SL}â‚‚(â„¤)$

$$
M =
\begin{pmatrix}
a & b \\
c & d
\end{pmatrix}
$$

Use $S$ to make $a, c$ positive.

Then use $Tâ»Â¹$ to reduce $a$ so $a < 0$ and $-a < c$.
Then flip them with $S$. This reduces $c$.
Repeat this process.

The final matrix is $\begin{pmatrix}
    1 & s \\
    0 & 1
\end{pmatrix}$ which is some power of $T$.
We now have a decomposition for $M$ by inverting the chain of operations.

# Every positive definite form is properly equivalent to a reduced form (theorem 6.14)

We already saw above that the smallest possible value for a reduced form is
$f(x, y) = a$.

## Algorithm

```python
if a > c or (a = c and b < 0):
    (a, b, c) â†’ (c, -b, a)                  #1
# Remaining two cases
elif a < c:
    if b <= -a:
        (a, b, c) â†’ (a, b + 2a, c + b + a)  #2
    else:
        assert b > a
        (a, b, c) â†’ (a, b - 2a, c - b + a)  #3
elif a = c and b >= 0:
    assert b > a
    (a, b, c) â†’ (a, b - 2a, c - b + a)      #4
```

First observe that in all the steps, $a$ does not increase.
Eventually it must become constant.

In the remaining two cases, the absolute value of $|b|$ gets smaller.
We will show that for each case.

### Branch 2: $b â‰¤ -a$

First assume $b = -a â‡’ |b| = a$, then we see that
$(a', b', c') = (a, a, c)$ and $b' = |b|$.
Now $a = b < c$ so the form is reduced.

Now assume $b < -a â‡’ a + b < 0 â‡’ 2a + b < a$.
But since $a > 0 â‡’ -a < 0$, we see
$b < -a < 0$.

If $2a + b > 0$ then
$|2a + b| = |b'| < a$. But $b < -a â‡’ a < |b| â‡’ |b'| < |b|$.

Else $b' = 2a + b < 0$, then
$a > 0, b < 0 â‡’ 2a + b > b$ so $|b'|$ also is smaller.

### Branch 3: $b > a$

$b > a$ and $a > 0 â‡’ 0 < a < b$.
$$ b - 2a < b $$

If $b - 2a â‰¥ 0$ then $|b - 2a| < |b|$ and we are done.

So now $b - 2a < 0$. Also $b > a â‡’ b - a > 0$.
We want to disprove $|b - 2a| â‰¥ |b|$.

First assume $|b - 2a| = |b|$, then $b > 0 â‡’ b - 2a = -b â‡’ a = 0$
which is impossible so $|b - 2a| > |b| = b$.
$$ â‡’ b - 2a < -b $$
$$ 2b - 2a < 0 $$
$$ b < a $$
which is a contradiction.

### Branch 4

The proof is essentially the same as branch 3, since $b > a$ and the transform
is the same.

## Determinant is Fixed

We can easily show algebraically the determinant is unchanged when applying any transform.
So $b'^2 - 4a'c' = bÂ² - 4ac$.

When $a = b$, then $c$ is also fixed.

# $ğ” = aâ„¤ + (b + cÏ‰)â„¤$ with $c|a$ and $c|b$

## $ğ” = âŸ¨a, b + cÏ‰âŸ©$

Let $m + nÏ‰ âˆˆ ğ”$

There is an $s$ such that
$$ n = sc + r \textrm{ with } r < c \textrm{ or } r = 0 $$
but $c$ is minimal so $r = 0$ and
$$ (m + nÏ‰) - s(b + cÏ‰) = m - sb $$
$b$ is chosen to be non-negative.

Now we have
$$ (m - sb) = ta + r_a $$
but $a$ is minimal so $r_a = 0$
$$ (m - sb) = (m + nÏ‰) - s(b + cÏ‰) $$
$$ â‡’ m + nÏ‰ = s(b + cÏ‰) + ta $$
$$ m + nÏ‰ âˆˆ aâ„¤ + (b + cÏ‰)â„¤ $$

## $c|a$

Since $c$ is minimal, we can use the same remainder trick to
prove $c|a$ and $c|b$
$$ a âˆˆ ğ” â‡’ aÏ‰ âˆˆ ğ” $$
$a = tc + r â‡’ aÏ‰ - t(b + cÏ‰) = -tb + rÏ‰$ with $r < c$, but
$c$ is minimal so $r = 0$ and $a = tc$.

## $c|b$

Likewise
$$ b + cÏ‰ âˆˆ ğ” â‡’ bÏ‰ + cd âˆˆ ğ” $$
again $b = tc + r$ so $(cd + bÏ‰) = t(b + cÏ‰) + ((-tb + cd) + rÏ‰) â‡’ r = 0$.

## $N_{K/â„š}(ğ”) = ac$

$$ M = [a, b + cÏ‰], \qquad S = \{ r + sÏ‰ : 0 â‰¤ r < a, 0 â‰¤ s < c \} $$
We prove $x + yÏ‰ âˆˆ â„¤_K$ is congruent mod $M$ to an element of $S$.

Let $y = cq + s$ where $q âˆˆ â„¤$ and $0 â‰¤ s < c$ then
$$ (x + yÏ‰) - q(b + cÏ‰) = x' + sÏ‰ $$
$$ â‡’ x + yÏ‰ â‰¡ x' + sÏ‰ \mod M $$
Now write $x' = aq' + r$ where $q' âˆˆ â„¤$ and $0 â‰¤ r < a$ then
$$ x' + sÏ‰ â‰¡ r + sÏ‰ \mod M $$
$$ N_{K/â„š}(ğ”) = \# S = ac $$

# $ac|cÂ²d - bÂ²$

Let $Î± âˆˆ ğ”$ then $Î±Ï‰ âˆˆ ğ”$
\begin{align*}
Î± &= ax + (b + cÏ‰)y \\
Î±Ï‰ &= cdy + (ax + by)Ï‰ \\
   &= as + (b + cÏ‰)t \quad \text{for some } s, t âˆˆ â„¤
\end{align*}
Comparing coefficients
\begin{align*}
as + bt &= cdy \\
ct &= ax + by \tag{1}
\end{align*}
$$ t = \frac{ax + by}{c} âˆˆ â„¤ â‡” c|a \text{ and } c|b $$
to see this choose $x, y = 0, 1$ or $1, 0$.

Combining (1) with $t$, and setting $x = 0$, we get that
$ac|cÂ²d - bÂ²$.

# $Î¦$

$$ Î¦ = \frac{N_{K/â„š}(ax + (b + cÏ‰)y)}{N_{K/â„š}(ğ”)} $$

$$ N_{K/â„š}(ax + by + cÏ‰y) = (ax + by)Â² - dcÂ²yÂ² $$
This is positive and so is $N_{K/â„š}(ğ”)$, so $Î¦(ğ”)$ is positive definite.

Let $Î± = a, Î² = b + cÏ‰$
\begin{align*}
N_{K/â„š}(Î±x + Î²y) &= (Î±x + Î²y)(\bar{Î±}x + \bar{Î²}y) \\
    &= N_{K/â„š}(Î±)xÂ² + T_{K/â„š}(Î±\bar{Î²})xy + N_{K/â„š}(Î²)yÂ²
\end{align*}

# Equivalence of Forms within Same Class
$$
F_{Î±, Î²} =
\begin{pmatrix}
Î± \\
Î²
\end{pmatrix}, \qquad
F_{Î³, Î´} =
\begin{pmatrix}
Î³ \\
Î´
\end{pmatrix}, \qquad
$$
$$ F_{Î±, Î²} = M F_{Î³, Î´} $$
$$ â‡’ \mathbf{v}^T F_{Î±, Î²} = \mathbf{v}^T M F_{Î³, Î´} $$
and also that
$$ \mathbf{v}^T F_{\bar{Î±}, \bar{Î²}} = \mathbf{v}^T M F_{\bar{Î³}, \bar{Î´}} $$

Also note that
$$ \mathbf{v}^T F = F^T \mathbf{v} \tag{1}$$

\begin{align*}
N_{K/â„š}(ğ”) Â· f_{Î±, Î²}(\mathbf{v}) &= N_{K/â„š}(ğ”) Â· f_{Î±, Î²}(x, y) = N_{K/â„š}(Î±x + Î²y) \\
    &= (Î±x + Î²y)(\bar{Î±}x + \bar{Î²}y) \\
    &= \mathbf{v}^T F_{Î±, Î²} \mathbf{v}^T F_{\bar{Î±}, \bar{Î²}} \\
    &= \mathbf{v}^T F_{Î±, Î²} F_{\bar{Î±}, \bar{Î²}}^T \mathbf{v} \qquad \text{by 1} \\
    &= \mathbf{v}^T M F_{Î³, Î´} (M F_{\bar{Î³}, \bar{Î´}})^T \mathbf{v} \\
    &= \mathbf{v}^T M F \bar{F}^T M^T \mathbf{v} \\
    &= (\mathbf{v}^T M) F (\mathbf{v}^T M) \bar{F} \\
    &= N_{K/â„š}(Î³(px + qy) + Î´(rx + sy)) \\
    &= N_{K/â„š}(ğ”) Â· f_{Î³, Î´}(px + qy, rx + sy)
\end{align*}

```python
sage: var("p r q s x y a b g d")
(p, r, q, s, x, y, a, b, g, d)
sage: v = matrix([[x], [y]])
sage: M = matrix([[p, r], [q, s]])
sage: vTM = v.transpose() * M
sage: vTM
[p*x + q*y r*x + s*y]
sage: F = matrix([[g], [d]])
sage: var("gb db")
(gb, db)
sage: Fb = matrix([[gb], [db]])
sage: vTM*F*vTM*Fb
[((r*x + s*y)*d + (p*x + q*y)*g)*(r*x + s*y)*db + ((r*x + s*y)*d + (p*x + q*y)*g)*(p*x + q*y)*gb]
sage: vTM*F*vTM*Fb == (g*(p*x + q*y) + d*(r*x + s*y))*(gb*(p*x + q*y) + db*(r*x + s*y))
True
```

# $ğ”$ and $ğ”Ÿ$ in the Same Ideal Class $â‡’ Î¦(ğ”) = Î¦(ğ”Ÿ)$ (Proposition 6.27)

*$ğ” \sim ğ”Ÿ â‡’ \frac{ğ”}{ğ”Ÿ} = âŸ¨Î¸âŸ©$ since the class group is defined modulo principal ideals.*

*There exists $Î¸ âˆˆ K$ such that $ğ”Ÿ = âŸ¨Î¸âŸ©ğ”$. Write $Î¸ = A/B$ for $A, B âˆˆ â„¤_K$.*

When $d < 0$ then $N_{K/â„š}(Î³) = |N_{K/â„š}(Î³)|$.
We will prove $Î¦(Î¼ğ”) = Î¦(ğ”)$.
Note $ğ” = â„¤Î± + â„¤Î²$.
\begin{align*}
f_{Î±, Î²} &= \frac{ N_{K/â„š}(Î±x + Î²y) }{ N_{K/â„š}(ğ”) } \\
f_{Î¼Î±, Î¼Î²} &= \frac{ N_{K/â„š}(Î¼Î±x + Î¼Î²y) }{ N_{K/â„š}(Î¼ğ”) } \\
           &= \frac{ N_{K/â„š}(Î¼) N_{K/â„š}(Î±x + Î²y) }{ N_{K/â„š}(âŸ¨Î¼âŸ©) N_{K/â„š}(ğ”) } \\
           &= \frac{ N_{K/â„š}(Î¼) N_{K/â„š}(Î±x + Î²y) }{ |N_{K/â„š}(Î¼)| N_{K/â„š}(ğ”) } \\
           &= \frac{ N_{K/â„š}(Î±x + Î²y) }{ N_{K/â„š}(ğ”) } \\
           &= f_{Î±, Î²} \\
\end{align*}
Since $ğ”Ÿ = \frac{A}{B}ğ” â‡’ Bğ”Ÿ = Ağ”$, then $Î¦(ğ”) = Î¦(Ağ”) = Î¦(Bğ”Ÿ) = Î¦(ğ”Ÿ)$.

# $d â‰¡ 1$ (mod 4)

## $ğ” = aâ„¤ + (b + cÏ)â„¤$ with $c|a$ and $c|b$

Same proof as before. Take $a$ and $b + cÏ$ where $a, c$ are minimal and positive.
Then subtract $m + nÏ$ to show there is an integer remainder.

Then $c|a$ because $a âˆˆ ğ” â‡’ aÏ âˆˆ ğ”$, meaning $aÏ - t(b + cÏ) â‡’ r = a - tc$ with either
$r < c$ or $r = 0$. But $c$ is minimal so $r = 0$ proving the statement.

Now we prove $c|b$.
Note $\bar{Ï} = \frac{\sqrt{d} - 1}{2} = Ï - 1$, and $Ï\bar{Ï} = \frac{d - 1}{4}$.
Then since $b + cÏ âˆˆ ğ”$,
$$ b\bar{Ï} + c\left(\frac{d - 1}{4}\right) = bÏ - b + c\left(\frac{d - 1}{4}\right) âˆˆ ğ” $$
Subtracting a multiple of $b + cÏ$, we see the coefficient for $Ï$
is $r = b - tc$ with $r = 0$ or $r < c$ but $c$ is minimal so $c | b$.

## $ac|cÂ²\left(\frac{d - 1}{4}\right) - bÂ² - bc$

\begin{align*}
Î±\bar{Ï} &= ax\bar{Ï} + by\bar{Ï} + cy\left(\frac{d - 1}{4}\right) \\
 &= (ax + by)Ï + (-ax -by + cy\left(\frac{d - 1}{4}\right)) \qquad \textrm{ since $\bar{Ï} = Ï - 1$} \\
 &= as + (b + cÏ)t
\end{align*}
Comparing coefficients for $Ï$ we see
\begin{align*}
ct &= ax + by \\
as + bt &= -ax -by + cy\left(\frac{d - 1}{4}\right) \\
â‡’ as &= -ax -by + cy\left(\frac{d - 1}{4}\right) - bt \\
    &= -ax -by + cy\left(\frac{d - 1}{4}\right) - bt \\
    &= -ax -by + cy\left(\frac{d - 1}{4}\right) - b\frac{ax + by}{c} \\
acs &= -acx -bcy + cÂ²y\left(\frac{d - 1}{4}\right) - b(ax + by) \\
\end{align*}
and since $c|b â‡’ ac|ab$
$$ ac|(-bc + cÂ²\left(\frac{d - 1}{4}\right) - bÂ²) $$

